
count(n) = count(n - 1) + count(n - 2) + count(n - 3)
count(n) : n段に到達するまでの組み合わせの数 = 答え


再帰
n = 0 : 1通り
n = 1 : 1通り
n = 2 : 2通り
n = 3 : 4通り (2 + 1 + 1)
n = 4 : 7通り (4 + 2 + 1)

...

n = k : count(k - 1) + count(k - 2) + count(k - 3)

f(n) = f(n - 1) + f(n - 2) + f(n - 3)
3^n


int count(int n) {
    if (memo[n] != null)
        return memo[n];

    switch (n){
        case 0:
        case 1:
            return 1;
        case 2:
            return 2;
        default:
            memo[n] = count(n - 1) + count(n - 2) + count(n -3);
            return memo[n]
    }
}


memo[n] = {0}
memo[0] = 1
memo[1] = 1
memo[2] = 2

for (int i = 3; i < n; i++) {
    memo[i] = memo[i - 1] + memo[i - 2] + memo[i - 3];
}

print(memo[n]);


for (int i = 0; i < n; i++) {
    memo[i + 1] += memo[i];
    memo[i + 2] += memo[i];
    memo[i + 3] += memo[i];
}



